Logic/Interpretability/PAHF/Coq/PAHFAdjoinTotal.v
@@ -364,6 +364,12 @@ Definition betaPrependPrefixCodeExistsTermAt :=
 Definition betaPrependPrefixCodeExistsTermAtBody :=
   PA.Formula.betaPrependPrefixCodeExistsTermAtBody.
 
+Definition betaPrependExistsTermAt :=
+  PA.Formula.betaPrependExistsTermAt.
+
+Definition betaPrependExistsTermAtBody :=
+  PA.Formula.betaPrependExistsTermAtBody.
+
 Definition betaPrependCodingStepTermAt :=
   PA.Formula.betaPrependCodingStepTermAt.
 
@@ -475,6 +481,36 @@ Proof.
   intros r sourceCode sourceStep head targetStep bound.
   exact (PA.Formula.rename_betaPrependPrefixCodeExistsTermAt
     r sourceCode sourceStep head targetStep bound).
+Qed.
+
+Lemma subst_betaPrependExistsTermAt :
+  forall sigma sourceCode sourceStep head bound,
+  subst sigma
+      (betaPrependExistsTermAt sourceCode sourceStep head bound) =
+    betaPrependExistsTermAt
+      (Term.subst sigma sourceCode)
+      (Term.subst sigma sourceStep)
+      (Term.subst sigma head)
+      (Term.subst sigma bound).
+Proof.
+  intros sigma sourceCode sourceStep head bound.
+  exact (PA.Formula.subst_betaPrependExistsTermAt
+    sigma sourceCode sourceStep head bound).
+Qed.
+
+Lemma rename_betaPrependExistsTermAt :
+  forall r sourceCode sourceStep head bound,
+  rename r
+      (betaPrependExistsTermAt sourceCode sourceStep head bound) =
+    betaPrependExistsTermAt
+      (Term.rename r sourceCode)
+      (Term.rename r sourceStep)
+      (Term.rename r head)
+      (Term.rename r bound).
+Proof.
+  intros r sourceCode sourceStep head bound.
+  exact (PA.Formula.rename_betaPrependExistsTermAt
+    r sourceCode sourceStep head bound).
 Qed.
 
 Lemma subst_betaPrependCodingStepTermAt :
@@ -1724,59 +1760,6 @@ Proof.
     (betaPrependPrefixCodeExistsTermAt
       sourceCode sourceStep head targetStep finalBound)
     himp (BProv_Ax_s_leTermAt_refl G finalBound)).
-Qed.
-
-Definition betaPrependExistsTermAt
-    (sourceCode sourceStep head bound : term) : formula :=
-  pEx (betaPrependPrefixCodeExistsTermAt
-    (Term.rename S sourceCode)
-    (Term.rename S sourceStep)
-    (Term.rename S head)
-    (tVar 0)
-    (Term.rename S bound)).
-
-Definition betaPrependExistsTermAtBody
-    (sourceCode sourceStep head bound : term) : formula :=
-  betaPrependPrefixCodeExistsTermAt
-    (Term.rename S sourceCode)
-    (Term.rename S sourceStep)
-    (Term.rename S head)
-    (tVar 0)
-    (Term.rename S bound).
-
-Lemma subst_betaPrependExistsTermAt :
-  forall sigma sourceCode sourceStep head bound,
-  subst sigma
-      (betaPrependExistsTermAt sourceCode sourceStep head bound) =
-    betaPrependExistsTermAt
-      (Term.subst sigma sourceCode)
-      (Term.subst sigma sourceStep)
-      (Term.subst sigma head)
-      (Term.subst sigma bound).
-Proof.
-  intros sigma sourceCode sourceStep head bound.
-  unfold betaPrependExistsTermAt.
-  cbn [subst].
-  rewrite subst_betaPrependPrefixCodeExistsTermAt.
-  repeat rewrite Term.subst_rename_succ_up.
-  reflexivity.
-Qed.
-
-Lemma rename_betaPrependExistsTermAt :
-  forall r sourceCode sourceStep head bound,
-  rename r
-      (betaPrependExistsTermAt sourceCode sourceStep head bound) =
-    betaPrependExistsTermAt
-      (Term.rename r sourceCode)
-      (Term.rename r sourceStep)
-      (Term.rename r head)
-      (Term.rename r bound).
-Proof.
-  intros r sourceCode sourceStep head bound.
-  rewrite <- subst_var_rename.
-  rewrite subst_betaPrependExistsTermAt.
-  repeat rewrite term_subst_var_rename.
-  reflexivity.
 Qed.
 
 Lemma BProv_Ax_s_betaPrependExistsTermAt_of_step :
